prove top-level correctness theorem in terms of the proof stubs in Api/Proofs.v

coq-verification/src/Concrete/Model.v
@@ -1,10 +1,13 @@
 Require Import Coq.Lists.List.
+Require Import Coq.Arith.PeanoNat.
 Require Import Hafnium.AbstractModel.
 Require Import Hafnium.Concrete.State.
 Require Import Hafnium.Concrete.Datatypes.
+Require Import Hafnium.Util.Tactics.
+Require Import Hafnium.Concrete.Api.Implementation.
+Require Import Hafnium.Concrete.Api.Proofs.
 Require Import Hafnium.Concrete.Assumptions.Addr.
 Require Import Hafnium.Concrete.Assumptions.Mpool.
-Require Import Hafnium.Concrete.Api.Implementation.
 
 (*** This file gives the definition of execution in the concrete model and
      includes the highest-level correctness proof, stating that the execution
@@ -15,20 +18,18 @@ Inductive api_call : Type :=
 | share_memory : nat -> ipaddr_t -> size_t -> hf_share -> vm -> api_call
 .
 
-Fixpoint execute_trace
-         {cp : concrete_params}
-         (start_state : concrete_state)
-         (trace : list api_call) : concrete_state :=
+Definition execute_trace
+           {cp : concrete_params}
+           (start_state : concrete_state)
+           (trace : list api_call) : concrete_state :=
   fold_right (fun next_call state =>
                 match next_call with
                 | clear_memory begin end_ ppool =>
-                  let '(_, state', _) :=
-                      api_clear_memory state begin end_ ppool in
-                  state'
+                  let ret := api_clear_memory state begin end_ ppool in
+                  snd (fst ret)
                 | share_memory vid addr size share current =>
-                  let '(_, state') :=
-                      api_share_memory state vid addr size share current in
-                  state'
+                  let ret := api_share_memory state vid addr size share current in
+                  snd ret
                 end)
              start_state trace.
 
@@ -40,13 +41,52 @@ Definition obeys_invariants
   exists abst : abstract_state,
     represents abst conc /\ AbstractModel.obeys_invariants abst.
 
+(* because [represents] includes [AbstractModel.is_valid], and we've proved all
+   valid abstract states obey the invariants, it's sufficient to just prove
+   [represents] *)
+Lemma represents_obeys_invariants
+      {ap : abstract_state_parameters} {cp : concrete_params}
+      (conc : concrete_state) :
+  (exists abst, represents abst conc) ->
+  obeys_invariants conc.
+Proof.
+  cbv [represents obeys_invariants]; basics.
+  eexists; basics; try solver; [ ].
+  apply (valid_obeys_invariants
+           (addr_eq_dec:=paddr_t_eq_dec) (vm_id_eq_dec:=Nat.eq_dec)).
+  eauto.
+Qed.
+
+Lemma execution_represents
+      {ap : abstract_state_parameters} {cp : concrete_params}
+      (start_state : concrete_state) (trace : list api_call) :
+  (exists abst, represents abst start_state) ->
+  exists abst, represents abst (execute_trace start_state trace).
+Proof.
+  cbv [execute_trace]; intros; induction trace; [ basics; solver | ].
+  destruct IHtrace as [abst IHtrace]. basics.
+  cbn [fold_right]. break_match.
+  { (* case : api_clear_memory *)
+    apply api_clear_memory_represents with (abst0:=abst).
+    eapply IHtrace. }
+  { (* case : api_share_memory *)
+    apply api_share_memory_represents with (abst0:=abst).
+    eapply IHtrace. }
+Qed.
+
 (*** Highest-level correctness theorem: any execution of api calls will preserve
      the invariants; that is, if you obey the invariants at the start, no
      sequence of api calls can make you stop obeying them. ***)
-Theorem execution_preserves_invariants :
-  forall {ap : abstract_state_parameters} {cp : concrete_params}
-         (start_state : concrete_state) (trace : list api_call),
+Theorem execution_preserves_invariants
+        {ap : abstract_state_parameters} {cp : concrete_params} :
+  forall (trace : list api_call) (start_state : concrete_state),
     obeys_invariants start_state ->
     obeys_invariants (execute_trace start_state trace).
 Proof.
-Admitted. (* TODO *)
+  intros; apply represents_obeys_invariants, execution_represents.
+  cbv [obeys_invariants] in *. basics; solver.
+Qed.
+
+(* Uncomment the below to see all assumptions that the top-level correctness
+   theorem depends on. *)
+(* Print Assumptions execution_preserves_invariants. *)
